CPGHelperML.thy
@@ -1,0 +1,64 @@
+theory CPGHelperML
+  imports ViperBoogieBasicRel
+begin
+
+ML \<open>
+fun unfold_bigblock_atomic ctxt bigblock =
+  case bigblock of
+    Const (bigblock_name, _) =>
+    ( let val thm = Proof_Context.get_thms ctxt (bigblock_name ^ "_def")
+      in
+         Local_Defs.unfold_tac ctxt thm
+      end )
+  | _ => all_tac
+ val test = @{term "BigBlock name [] None None"}
+
+fun is_empty_bigblock bigblock =
+  case bigblock of 
+   Const (@{const_name BigBlock}, _) 
+   $ _ (* name *)
+   $ Const (@{const_name Nil}, _)
+   $ Const (@{const_name None}, _)
+   $ Const (@{const_name None}, _)
+    => true
+  | _ => false
+
+fun unfold_bigblock_in_program_point ctxt (program_point, _) =
+    case program_point of 
+     Const (@{const_name Product_Type.Pair}, _) $ bigblock $ cont =>
+        if is_empty_bigblock bigblock then
+           (case cont of (* if the current big block is empty, we unfold the next big block *)
+              Const (@{const_name KSeq}, _) $ bigblock_in_cont $ _ => 
+                unfold_bigblock_atomic ctxt bigblock_in_cont
+            | _ => all_tac)
+        else
+          unfold_bigblock_atomic ctxt bigblock        
+     | _ => all_tac   
+
+(* input term t should not have any metaimplications or metaquantifications *)
+fun unfold_bigblock_in_goal_aux ctxt (t,i) =
+  case t of 
+    @{term "Trueprop"} $ t' => unfold_bigblock_in_goal_aux ctxt (t',i)
+  | @{term "(\<and>)"} $ conj1 $ _ => (unfold_bigblock_in_goal_aux ctxt (conj1, i))
+  | Const (@{const_name "red_ast_bpl"}, _) 
+         $ _ (* AST *)
+         $ _ (* econtext_bpl *)
+         $ (Const (@{const_name Product_Type.Pair}, _) $ program_point $ _)
+         $ _ (* end config *) =>
+            unfold_bigblock_in_program_point ctxt (program_point, i)
+  | Const (@{const_name "is_empty_bigblock"}, _) $ bigblock =>
+      unfold_bigblock_atomic ctxt bigblock
+  | _ => (writeln(Syntax.string_of_term ctxt t); all_tac)
+  
+
+(* The following tactic unfolds in certain contexts the currently active bigblock or the next 
+bigblock if the currently active bigblock is empty.
+The goal is to make sure that after this tactic the (bigblock, continuation) configuration is in 
+a form where bigblock is unfolded and not empty. The nonemptiness guarantee relies on the assumption
+ that an empty bigblocks is not succeeded by another empty bigblock. *)
+fun unfold_bigblock_in_goal ctxt =
+  SUBGOAL (fn (t,i) => unfold_bigblock_in_goal_aux ctxt (Logic.strip_assums_concl t, i))
+\<close>
+
+
+end
