ExprWfRelML.thy
@@ -1,11 +1,23 @@
 theory ExprWfRelML
-imports ExprWfRel ExpRelML TotalViperHelperML Boogie_Lang.HelperML
+imports ExprWfRel ExpRelML TotalViperHelperML Boogie_Lang.HelperML TotalViper.CPGHelperML
 begin
 
 ML \<open>
-
   val R' = run_and_print_if_fail_tac' "failure"
   val Rmsg' = run_and_print_if_fail_tac' 
+
+  fun progress_tac ctxt = 
+     (*(asm_full_simp_tac ctxt ORELSE' (K all_tac)) THEN'*)  (* simplify continuation *)
+      
+     resolve_tac ctxt [@{thm exI}] THEN'
+     resolve_tac ctxt [@{thm conjI}] THEN'
+    (* (K (print_tac ctxt "before unfold"))  THEN'*)
+     (unfold_bigblock_in_goal ctxt) THEN'
+    (* (K (print_tac ctxt "after unfold"))  THEN' *)
+     (resolve_tac ctxt [@{thm red_ast_bpl_refl}] ORELSE' 
+      
+      resolve_tac ctxt [@{thm red_ast_bpl_empty_block}]) THEN'
+     assm_full_simp_solved_tac ctxt
 
   fun exp_wf_rel_trivial_tac ctxt =
       FIRST' [
@@ -40,6 +52,10 @@ ML \<open>
 
   
   fun bop_wf_rel_div_mod exp_rel_info ctxt = 
+      (* need to first progress the configuration in case the currently active bigblock is not unfolded or
+         if the current bigblock is empty *)
+      resolve_tac ctxt [@{thm wf_rel_extend_2}] THEN' 
+      progress_tac ctxt THEN'
       resolve_tac ctxt [@{thm syn_bop_op_non_trivial_wf_rel}] THEN'
       (Rmsg' "div_rel_1" assm_full_simp_solved_tac ctxt) (* bop *) THEN'
       (exp_rel_tac exp_rel_info ctxt |> SOLVED') THEN'
@@ -62,16 +78,9 @@ ML \<open>
       assm_full_simp_solved_tac ctxt, (* bop *)
       
       bop_wf_rel_div_mod exp_rel_info ctxt |> SOLVED'
-   ]
-        
-  fun progress_tac ctxt = 
-     (asm_full_simp_tac ctxt ORELSE' (K all_tac)) THEN'  (* simplify continuation *)
-     resolve_tac ctxt [@{thm exI}] THEN'
-     resolve_tac ctxt [@{thm conjI}] THEN'     
-     (resolve_tac ctxt [@{thm red_ast_bpl_refl}] ORELSE' 
-      resolve_tac ctxt [@{thm red_ast_bpl_empty_block}]) THEN'
-     assm_full_simp_solved_tac ctxt
-
+   ]      
+  
+  fun simplify_continuation ctxt = asm_full_simp_tac ctxt
 
   fun exp_wf_rel_non_trivial_tac exp_rel_info ctxt = 
      FIRST_AND_THEN' [
@@ -97,13 +106,20 @@ ML \<open>
    and 
       binop_lazy_wf_rel_tac exp_rel_info ctxt =   
         (
-         (exp_wf_rel_non_trivial_tac exp_rel_info ctxt |> SOLVED') THEN' (* e1 *)
-         (Rmsg' "Lazy1" progress_tac ctxt) THEN' (* progress to if *)        
+         (Rmsg' "Wf E1" (exp_wf_rel_non_trivial_tac exp_rel_info) ctxt |> SOLVED') THEN' (* e1 *)
+         (Rmsg' "Lazy1" progress_tac ctxt) THEN' (* progress to if *) 
+         (Rmsg' "LazyEmptyElse" (* empty else block *)
+                (fn ctxt => 
+                   (unfold_bigblock_in_goal ctxt) THEN'
+                   (assm_full_simp_solved_tac ctxt)
+                )
+                ctxt) THEN'
          (Rmsg' "Lazy2" assm_full_simp_solved_tac ctxt) THEN' (* guard And/Imp *)
          (Rmsg' "Lazy3" assm_full_simp_solved_tac ctxt) THEN' (* guard Or *)
          ((Rmsg' "Lazy4" (exp_rel_tac exp_rel_info) ctxt) |> SOLVED') THEN' (* e1 exp rel *)
-         (exp_wf_rel_non_trivial_tac exp_rel_info ctxt |> SOLVED') THEN' (* e2 *)
-         (progress_tac ctxt |> SOLVED') (* progress to expected configuration *)
+         (Rmsg' "Simplify Cont" simplify_continuation ctxt) THEN' (* simplify continuation since we introduce convert_list_to_cont *)
+         (Rmsg' "Wf E2" (exp_wf_rel_non_trivial_tac exp_rel_info) ctxt |> SOLVED') THEN' (* e2 *)
+         (Rmsg' "Progress2" progress_tac ctxt |> SOLVED')  (* progress to expected configuration *)
         )
     
 (*
