TotalViperHelperML.thy
@@ -7,7 +7,7 @@ fun run_and_print_if_fail_tac tac ctxt =
     (tac ctxt) ORELSE (print_tac ctxt "failure" THEN no_tac)
 
 fun run_and_print_if_fail_tac' msg tac ctxt =
-    (tac ctxt) ORELSE' (K ( (print_tac ctxt msg) THEN no_tac) )
+    (tac ctxt) ORELSE' (K ((print_tac ctxt msg) THEN no_tac))
 \<close>
 
 end
